code/rsapss/Hacl.Bignum.Exponentiation.fst
@@ -7,9 +7,10 @@ open FStar.Mul
 open Lib.IntTypes
 open Lib.Buffer
 
+module BN = Hacl.Bignum
+module BM = Hacl.Bignum.Montgomery
+
 open Hacl.Bignum.Definitions
-open Hacl.Bignum
-open Hacl.Bignum.Montgomery
 
 module ST = FStar.HyperStack.ST
 module S = Hacl.Spec.Bignum.Exponentiation
@@ -19,10 +20,10 @@ friend Hacl.Spec.Bignum.Exponentiation
 
 #reset-options "--z3rlimit 50 --fuel 0 --ifuel 0"
 
-val bn_mod_exp_:
-    nLen:size_t
-  -> rLen:size_t{v rLen = v nLen + 1 /\ v rLen + v rLen <= max_size_t}
-  -> n:lbignum nLen
+inline_for_extraction noextract
+let bn_mod_exp_loop_st (nLen: BN.meta_len) =
+  let rLen = nLen +. 1ul in
+    n:lbignum nLen
   -> nInv_u64:uint64
   -> bBits:size_t{v bBits > 0}
   -> bLen:size_t{v bLen = v (blocks bBits 64ul) /\ (v bBits - 1) / 64 < v bLen}
@@ -40,17 +41,23 @@ val bn_mod_exp_:
 	(S.bn_mod_exp_f (as_seq h0 n) nInv_u64 (v bBits) (v bLen) (as_seq h0 b))
       (as_seq h0 aM, as_seq h0 accM))
 
+val bn_mod_exp_loop: nLen:BN.meta_len
+  -> (#[FStar.Tactics.Typeclasses.tcresolve ()] _ : Hacl.Bignum.Montgomery.mont nLen)
+  -> bn_mod_exp_loop_st nLen
+
 [@CInline]
-let bn_mod_exp_ nLen rLen n nInv_u64 bBits bLen b aM accM =
+let bn_mod_exp_loop nLen #_ n nInv_u64 bBits bLen b aM accM =
+  [@ inline_let]
+  let rLen = nLen +. 1ul in
   [@inline_let]
   let spec h0 = S.bn_mod_exp_f (as_seq h0 n) nInv_u64 (v bBits) (v bLen) (as_seq h0 b) in
   let h0 = ST.get () in
   loop2 h0 bBits aM accM spec
   (fun i ->
     Lib.LoopCombinators.unfold_repeati (v bBits) (spec h0) (as_seq h0 aM, as_seq h0 accM) (v i);
-    (if (bn_is_bit_set bLen b i) then
-      mont_mul nLen rLen n nInv_u64 aM accM accM); // acc = (acc * a) % n
-    mont_mul nLen rLen n nInv_u64 aM aM aM // a = (a * a) % n
+    if BN.bn_is_bit_set bLen b i then
+      BM.mul n nInv_u64 aM accM accM; // acc = (acc * a) % n
+    BM.mul n nInv_u64 aM aM aM // a = (a * a) % n
   )
 
 
@@ -58,6 +65,8 @@ inline_for_extraction noextract
 val bn_mod_exp_mont:
     modBits:size_t{v modBits > 0}
   -> nLen:size_t{0 < v nLen /\ 128 * (v nLen + 1) <= max_size_t /\ v nLen == v (blocks modBits 64ul)}
+  -> (#[FStar.Tactics.Typeclasses.tcresolve ()] _ : Hacl.Bignum.Montgomery.mont nLen)
+  -> bn_mod_exp_loop:bn_mod_exp_loop_st nLen
   -> n:lbignum nLen
   -> a:lbignum nLen
   -> acc:lbignum nLen
@@ -72,29 +81,43 @@ val bn_mod_exp_mont:
   (ensures  fun h0 _ h1 -> modifies (loc res) h0 h1 /\
     as_seq h1 res == S.bn_mod_exp_mont (v modBits) (v nLen) (as_seq h0 n) (as_seq h0 a) (as_seq h0 acc) (v bBits) (as_seq h0 b))
 
-let bn_mod_exp_mont modBits nLen n a acc bBits b res =
+let bn_mod_exp_mont modBits nLen #_ bn_mod_exp_loop n a acc bBits b res =
   push_frame ();
   let rLen = nLen +! 1ul in
   let bLen = blocks bBits 64ul in
-  let nInv_u64 = mod_inv_u64 n.(0ul) in // n * nInv = 1 (mod (pow2 64))
+  let nInv_u64 = BM.mod_inv_u64 n.(0ul) in // n * nInv = 1 (mod (pow2 64))
 
   let r2 = create nLen (u64 0) in
-  precomp_r2_mod_n nLen modBits n r2;
+  BM.precomp modBits n r2;
 
   let aM   = create rLen (u64 0) in
   let accM = create rLen (u64 0) in
-  to_mont nLen rLen n nInv_u64 r2 a aM;
-  to_mont nLen rLen n nInv_u64 r2 acc accM;
-  bn_mod_exp_ nLen rLen n nInv_u64 bBits bLen b aM accM;
-  from_mont nLen rLen n nInv_u64 accM res;
-  bn_sub_mask nLen n res;
+  BM.to n nInv_u64 r2 a aM;
+  BM.to n nInv_u64 r2 acc accM;
+  bn_mod_exp_loop n nInv_u64 bBits bLen b aM accM;
+  BM.from n nInv_u64 accM res;
+  // Note here that type class resolution looks up in the parent type class.
+  BN.sub_mask n res;
   pop_frame ()
 
 
+inline_for_extraction noextract
+val mk_bn_mod_exp:
+    modBits:size_t{v modBits > 0}
+  -> nLen:size_t{0 < v nLen /\ 128 * (v nLen + 1) <= max_size_t /\ v nLen == v (blocks modBits 64ul)}
+  -> (#[FStar.Tactics.Typeclasses.tcresolve ()] _ : Hacl.Bignum.Montgomery.mont nLen)
+  -> bn_mod_exp_loop:bn_mod_exp_loop_st nLen ->
+  bn_mod_exp_st modBits nLen
+
 [@CInline]
-let bn_mod_exp modBits nLen n a bBits b res =
+let mk_bn_mod_exp modBits nLen #_ bn_mod_exp_loop n a bBits b res =
   push_frame ();
   let acc  = create nLen (u64 0) in
   acc.(0ul) <- u64 1;
-  bn_mod_exp_mont modBits nLen n a acc bBits b res;
+  bn_mod_exp_mont modBits nLen bn_mod_exp_loop n a acc bBits b res;
   pop_frame ()
+
+let bn_mod_exp modBits nLen =
+  [@ inline_let ]
+  let inst = BM.mk_runtime_mont nLen in
+  mk_bn_mod_exp modBits nLen (bn_mod_exp_loop nLen #inst)
