code/rsapss/Hacl.Bignum.Exponentiation.fsti
@@ -11,13 +11,12 @@ open Hacl.Bignum.Definitions
 
 module S = Hacl.Spec.Bignum.Exponentiation
 
-
 #reset-options "--z3rlimit 50 --fuel 0 --ifuel 0"
 
-val bn_mod_exp:
-    modBits:size_t{v modBits > 0}
-  -> nLen:size_t{0 < v nLen /\ v nLen = v (blocks modBits 64ul) /\ 128 * (v nLen + 1) <= max_size_t}
-  -> n:lbignum nLen
+let bn_mod_exp_st (modBits:size_t{v modBits > 0})
+  (nLen:size_t{0 < v nLen /\ v nLen = v (blocks modBits 64ul) /\ 128 * (v nLen + 1) <= max_size_t})
+=
+    n:lbignum nLen
   -> a:lbignum nLen
   -> bBits:size_t{v bBits > 0}
   -> b:lbignum (blocks bBits 64ul)
@@ -28,3 +27,6 @@ val bn_mod_exp:
     disjoint res a /\ disjoint res b /\ disjoint res n /\ disjoint n a)
   (ensures  fun h0 _ h1 -> modifies (loc res) h0 h1 /\
     as_seq h1 res == S.bn_mod_exp (v modBits) (v nLen) (as_seq h0 n) (as_seq h0 a) (v bBits) (as_seq h0 b))
+
+// This version is fully run-time.
+val bn_mod_exp: modBits:_ -> nLen:_ -> bn_mod_exp_st modBits nLen
