code/rsapss/Hacl.Bignum.Montgomery.fst
@@ -9,7 +9,6 @@ open Lib.Buffer
 
 open Hacl.Bignum.Definitions
 open Hacl.Bignum.Base
-open Hacl.Bignum
 open Hacl.Impl.Lib
 
 module ST = FStar.HyperStack.ST
@@ -18,6 +17,8 @@ module LSeq = Lib.Sequence
 
 module S = Hacl.Spec.Bignum.Montgomery
 module SB = Hacl.Spec.Bignum
+
+module BN = Hacl.Bignum
 
 friend Hacl.Spec.Bignum.Montgomery
 
@@ -75,9 +76,12 @@ let mod_inv_u64 n0 =
   pop_frame ();
   res
 
-let precomp_r2_mod_n nLen modBits n res =
+let precomp_r2_mod_n #nLen #_ modBits n res =
   memset res (u64 0) nLen;
-  bn_bit_set nLen res (modBits -! 1ul);
+  // Note here that BN.bit_set refers to the implicitly-defined projector for
+  // the type class rather than the bn_bit_set operator. So we're really
+  // selecting the implementation of bn_bit_set specialized for nLen!
+  BN.bit_set res (modBits -! 1ul);
 
   [@inline_let]
   let spec h = S.bn_lshift1_mod_n (as_seq h n) in
@@ -86,7 +90,7 @@ let precomp_r2_mod_n nLen modBits n res =
   loop1 h0 (128ul *! nLen +! 129ul -! modBits) res spec
   (fun i ->
     Loops.unfold_repeati (128 * v nLen + 129 - v modBits) (spec h0) (as_seq h0 res) (v i);
-    bn_add_mod_n nLen n res res res
+    BN.add_mod_n n res res res
   )
 
 
@@ -106,19 +110,24 @@ val mont_reduction_f:
 let mont_reduction_f nLen rLen n nInv_u64 j res =
   push_frame ();
   let qj = nInv_u64 *. res.(j) in
-  let c = bn_mul1_lshift_add_in_place nLen n qj (rLen +! rLen) j res in
+  // Keeping the inline_for_extraction version here.
+  let c = BN.bn_mul1_lshift_add_in_place nLen n qj (rLen +! rLen) j res in
   let c = create 1ul c in
 
   let h0 = ST.get () in
   let res2 = sub res (j +! nLen) (rLen +! rLen -! j -! nLen) in
   let _ = update_sub_f_carry #uint64 #carry h0 res (j +! nLen) (rLen +! rLen -! j -! nLen)
     (fun h -> SB.bn_add (as_seq h0 res2) (as_seq h0 c))
-    (fun _ -> bn_add (rLen +! rLen -! j -! nLen) res2 1ul c res2) in
+    // Also keeping the inline_for_extraction version, since the nLen parameter
+    // is too complicated to specialize ahead-of-time.
+    (fun _ -> BN.bn_add (rLen +! rLen -! j -! nLen) res2 1ul c res2) in
   pop_frame ()
 
 
 [@CInline]
-let mont_reduction nLen rLen n nInv_u64 c res =
+let mont_reduction nLen n nInv_u64 c res =
+  [@ inline_let]
+  let rLen = nLen +. 1ul in
   [@ inline_let]
   let spec h = S.mont_reduction_f #(v nLen) #(v rLen) (as_seq h n) nInv_u64 in
 
@@ -128,11 +137,15 @@ let mont_reduction nLen rLen n nInv_u64 c res =
     Loops.unfold_repeati (v rLen) (spec h0) (as_seq h0 c) (v j);
     mont_reduction_f nLen rLen n nInv_u64 j c
   );
-  bn_rshift (rLen +! rLen) c rLen res
+  // Easy to specialize, but such a small function that it's not worth it (per
+  // Marina's advice).
+  BN.bn_rshift (rLen +! rLen) c rLen res
 
 
 [@CInline]
-let to_mont nLen rLen n nInv_u64 r2 a aM =
+let to_mont #nLen #_ n nInv_u64 r2 a aM =
+  [@ inline_let]
+  let rLen = nLen +. 1ul in
   push_frame ();
   let tmp = create (rLen +! rLen) (u64 0) in
 
@@ -140,26 +153,32 @@ let to_mont nLen rLen n nInv_u64 r2 a aM =
   let c = sub tmp 0ul (nLen +! nLen) in
   update_sub_f h0 tmp 0ul (nLen +! nLen)
     (fun h -> SB.bn_mul (as_seq h0 a) (as_seq h0 r2))
-    (fun _ -> bn_mul nLen a nLen r2 c);
-  mont_reduction nLen rLen n nInv_u64 tmp aM; // aM = c % n
+    (fun _ -> BN.mul a r2 c);
+  mont_reduction nLen n nInv_u64 tmp aM; // aM = c % n
   pop_frame ()
 
 
 [@CInline]
-let from_mont nLen rLen n nInv_u64 aM a =
+let from_mont #nLen mont_reduction n nInv_u64 aM a =
+  [@ inline_let]
+  let rLen = nLen +. 1ul in
   push_frame ();
   let tmp = create (rLen +! rLen) (u64 0) in
   update_sub tmp 0ul rLen aM;
   let a' = create rLen (u64 0) in
-  mont_reduction nLen rLen n nInv_u64 tmp a';
+  mont_reduction n nInv_u64 tmp a';
   copy a (sub a' 0ul nLen);
   pop_frame ()
 
 
 [@CInline]
-let mont_mul nLen rLen n nInv_u64 aM bM resM =
+let mont_mul #nLen #k mont_reduction n nInv_u64 aM bM resM =
+  [@ inline_let]
+  let rLen = nLen +. 1ul in
   push_frame ();
   let c = create (rLen +! rLen) (u64 0) in
-  bn_mul rLen aM rLen bM c; // c = aM * bM
-  mont_reduction nLen rLen n nInv_u64 c resM; // resM = c % n
+  // In case you need to debug the type class projection, this is the explicit
+  // syntax without referring to the implicitly-defined projector.
+  k.BN.mul' aM bM c; // c = aM * bM
+  mont_reduction n nInv_u64 c resM; // resM = c % n
   pop_frame ()
