code/rsapss/Hacl.Bignum.Montgomery.fsti
@@ -9,6 +9,7 @@ open Lib.Buffer
 
 open Hacl.Bignum.Definitions
 module S = Hacl.Spec.Bignum.Montgomery
+module BN = Hacl.Bignum
 
 
 #reset-options "--z3rlimit 50 --fuel 0 --ifuel 0"
@@ -19,10 +20,9 @@ val mod_inv_u64: n0:uint64 ->
   (ensures  fun h0 r h1 -> modifies0 h0 h1 /\
     r == S.mod_inv_u64 n0)
 
-
-val precomp_r2_mod_n:
-    nLen:size_t{0 < v nLen /\ 128 * (v nLen + 1) <= max_size_t}
-  -> modBits:size_t{0 < v modBits /\ v nLen == v (blocks modBits 64ul)}
+inline_for_extraction noextract
+let precomp_r2_mod_n_st (nLen: BN.meta_len) =
+    modBits:size_t{0 < v modBits /\ v nLen == v (blocks modBits 64ul)}
   -> n:lbignum nLen
   -> res:lbignum nLen ->
   Stack unit
@@ -30,11 +30,19 @@ val precomp_r2_mod_n:
   (ensures  fun h0 _ h1 -> modifies (loc res) h0 h1 /\
     as_seq h1 res == S.precomp_r2_mod_n (v modBits) (as_seq h0 n))
 
+// Not marking this one as noextract, since it legitimately can execute with
+// nLen passed at run-time. It's just a little inefficient. (And it's helpful to
+// keep a super-generic bignum implementation for any width.)
+val precomp_r2_mod_n:
+    #nLen:BN.meta_len
+  -> (#[FStar.Tactics.Typeclasses.tcresolve ()] _ : BN.bn nLen)
+  -> precomp_r2_mod_n_st nLen
 
-val mont_reduction:
-    nLen:size_t
-  -> rLen:size_t{v rLen = v nLen + 1 /\ v rLen + v rLen <= max_size_t}
-  -> n:lbignum nLen
+
+inline_for_extraction noextract
+let mont_reduction_st (nLen:size_t { v nLen + 1 + v nLen + 1 <= max_size_t }) =
+  let rLen = nLen +. 1ul in
+    n:lbignum nLen
   -> mu:uint64
   -> c:lbignum (rLen +! rLen)
   -> res:lbignum rLen ->
@@ -45,11 +53,15 @@ val mont_reduction:
   (ensures  fun h0 _ h1 -> modifies (loc res |+| loc c) h0 h1 /\
     as_seq h1 res == S.mont_reduction #(v nLen) #(v rLen) (as_seq h0 n) mu (as_seq h0 c))
 
+val mont_reduction:
+    nLen:BN.meta_len
+  -> mont_reduction_st nLen
 
-val to_mont:
-    nLen:size_t
-  -> rLen:size_t{v rLen = v nLen + 1 /\ v rLen + v rLen <= max_size_t}
-  -> n:lbignum nLen
+
+inline_for_extraction noextract
+let to_mont_st (nLen: BN.meta_len) =
+  let rLen = nLen +. 1ul in
+    n:lbignum nLen
   -> mu:uint64
   -> r2:lbignum nLen
   -> a:lbignum nLen
@@ -62,11 +74,16 @@ val to_mont:
   (ensures  fun h0 _ h1 -> modifies (loc aM) h0 h1 /\
     as_seq h1 aM == S.to_mont #(v nLen) #(v rLen) (as_seq h0 n) mu (as_seq h0 r2) (as_seq h0 a))
 
+val to_mont:
+    #nLen:BN.meta_len
+  -> (#[FStar.Tactics.Typeclasses.tcresolve ()] _ : BN.bn nLen)
+  -> to_mont_st nLen
 
-val from_mont:
-    nLen:size_t
-  -> rLen:size_t{v rLen = v nLen + 1 /\ v rLen + v rLen <= max_size_t}
-  -> n:lbignum nLen
+
+inline_for_extraction noextract
+let from_mont_st (nLen: BN.meta_len) =
+  let rLen = nLen +. 1ul in
+    n:lbignum nLen
   -> mu:uint64
   -> aM:lbignum rLen
   -> a:lbignum nLen ->
@@ -77,11 +94,18 @@ val from_mont:
   (ensures  fun h0 _ h1 -> modifies (loc a) h0 h1 /\
     as_seq h1 a == S.from_mont #(v nLen) #(v rLen) (as_seq h0 n) mu (as_seq h0 aM))
 
+// This one just needs a specialized implementation of mont_reduction. No point
+// in doing a type class for a single function , so we take it as a parameter.
+val from_mont:
+    #nLen:BN.meta_len
+  -> mr: mont_reduction_st nLen
+  -> from_mont_st nLen
 
-val mont_mul:
-    nLen:size_t
-  -> rLen:size_t{v rLen = v nLen + 1 /\ v rLen + v rLen <= max_size_t}
-  -> n:lbignum nLen
+
+inline_for_extraction noextract
+let mont_mul_st (nLen: BN.meta_len) =
+  let rLen = nLen +. 1ul in
+    n:lbignum nLen
   -> mu:uint64
   -> aM:lbignum rLen
   -> bM:lbignum rLen
@@ -93,3 +117,39 @@ val mont_mul:
     eq_or_disjoint aM resM /\ eq_or_disjoint bM resM)
   (ensures  fun h0 _ h1 -> modifies (loc resM) h0 h1 /\
     as_seq h1 resM == S.mont_mul (as_seq h0 n) mu (as_seq h0 aM) (as_seq h0 bM))
+
+/// This one needs both the type class and a specialized montgomery reduction.
+val mont_mul:
+    #nLen:BN.meta_len
+  -> (#[FStar.Tactics.Typeclasses.tcresolve ()] _ : BN.bn nLen)
+  -> mr: mont_reduction_st nLen
+  -> mont_mul_st nLen
+
+
+/// A montgomery implementation specialized for a bignum length.
+inline_for_extraction noextract
+class mont (len: BN.meta_len)  = {
+  bn: BN.bn len;
+  precomp: precomp_r2_mod_n_st len;
+  reduction: mont_reduction_st len;
+  to: to_mont_st len;
+  from: from_mont_st len;
+  mul: mont_mul_st len;
+}
+
+/// Encoding type-class hierarchies via a hook for type class resolution.
+inline_for_extraction noextract
+instance bn_of_mont (#len: BN.meta_len) (x: mont len): BN.bn len = x.bn
+
+// Same here: a completely run-time-only instance.
+// FIXME: I cannot seem to use any dependency and must repeat the definitions of
+// bn and reduction.
+inline_for_extraction noextract
+let mk_runtime_mont (len: BN.meta_len): mont len = {
+  bn = BN.mk_runtime_bn len;
+  precomp = norm [ zeta; primops; iota; delta_only [`%precomp_r2_mod_n;] ] (precomp_r2_mod_n #len #(BN.mk_runtime_bn len));
+  reduction = mont_reduction len;
+  to = to_mont #len #(BN.mk_runtime_bn len);
+  from = from_mont #len (mont_reduction len);
+  mul = mont_mul #len #(BN.mk_runtime_bn len) (mont_reduction len);
+}
