code/rsapss/Hacl.Bignum4096.fst
@@ -1,0 +1,83 @@
+module Hacl.Bignum4096
+
+open FStar.Mul
+
+module BN = Hacl.Bignum
+module BM = Hacl.Bignum.Montgomery
+module BE = Hacl.Bignum.Exponentiation
+
+friend Hacl.Bignum.Exponentiation
+
+let _ = assert_norm (4096ul = 64ul `FStar.UInt32.mul` 64ul)
+
+inline_for_extraction noextract
+let n': BN.meta_len = 65ul
+
+/// A note about the style of normalization used in this file. Normally,
+/// bn_sub_eq_len and others would be marked as inline_for_extraction. However,
+/// we want to keep a copy of the functions that take the nLen parameter at
+/// runtime, meaning we can't blindly mark everything as inline_for_extraction,
+/// otherwise the copy of the code that a runtime-parametric over the length
+/// would be horrendous. So instead we do the inline_by_extraction "by hand" via
+/// a call to `norm`. Note that these are all partial applications, meaning that
+/// we normalize pure terms.
+
+
+let add = Hacl.Bignum.Addition.bn_add_eq_len n
+
+let sub = Hacl.Bignum.Addition.bn_sub_eq_len n
+
+let mul (a b: lbignum n): BN.bn_mul_st a b =
+  norm [ delta; zeta; primops; iota; delta_only [ `%BN.bn_mul; `%Hacl.Bignum.Multiplication.bn_mul ] ] (BN.bn_mul n a n b)
+
+let bit_set: BN.bn_bit_set_st n =
+  BN.(norm [ zeta; primops; iota; delta_only [ `%bn_bit_set ] ] (bn_bit_set n))
+
+let add_mod_n: BN.bn_add_mod_n_st n =
+  BN.bn_add_mod_n n
+
+let sub_mask: BN.bn_sub_mask_st n =
+  BN.bn_sub_mask n
+
+let mul' (a b: lbignum n'): BN.bn_mul_st a b =
+  norm [ zeta; primops; iota; delta_only [ `%BN.bn_mul; `%Hacl.Bignum.Multiplication.bn_mul ] ] (BN.bn_mul n' a n' b)
+
+inline_for_extraction noextract
+instance bn_inst: BN.bn n = {
+  BN.bit_set;
+  BN.add_mod_n;
+  BN.mul;
+  BN.mul';
+  BN.sub_mask
+}
+
+let precomp: BM.precomp_r2_mod_n_st n =
+  BM.(norm [ zeta; primops; iota; delta_only [`%precomp_r2_mod_n;] ] (precomp_r2_mod_n #n #bn_inst))
+
+let reduction: BM.mont_reduction_st n =
+  BM.(norm [ zeta; primops; iota; delta_only [ `%mont_reduction ] ] (mont_reduction n))
+
+let to: BM.to_mont_st n =
+  BM.(norm [ zeta; primops; iota; delta_only [ `%to_mont ] ] (to_mont #n #bn_inst))
+
+let from: BM.from_mont_st n =
+  norm [ zeta; primops; iota; delta_only [ `%BM.from_mont ] ] (BM.from_mont #n reduction)
+
+let mont_mul: BM.mont_mul_st n =
+  norm [ zeta; primops; iota; delta_only [ `%BM.mont_mul ] ] (BM.mont_mul #n #bn_inst reduction)
+
+inline_for_extraction noextract
+instance mont_inst: BM.mont n = {
+  BM.bn = FStar.Tactics.Typeclasses.solve;
+  BM.precomp;
+  BM.reduction;
+  BM.to;
+  BM.from;
+  BM.mul = mont_mul;
+}
+
+let mod_exp_loop: BE.bn_mod_exp_loop_st n =
+  norm [ zeta; primops; iota; delta_only [ `%BE.bn_mod_exp_loop ] ] (BE.bn_mod_exp_loop n #mont_inst)
+
+let mod_exp =
+  BE.mk_bn_mod_exp 4096ul n #mont_inst mod_exp_loop
