code/rsapss/Hacl.Bignum4096.fsti
@@ -1,0 +1,37 @@
+module Hacl.Bignum4096
+
+open FStar.Mul
+
+module BN = Hacl.Bignum
+module BM = Hacl.Bignum.Montgomery
+module BE = Hacl.Bignum.Exponentiation
+
+let _ = assert_norm (4096ul = 64ul `FStar.UInt32.mul` 64ul)
+
+inline_for_extraction noextract
+let n: BN.meta_len = 64ul
+
+inline_for_extraction noextract
+let lbignum = Hacl.Bignum.Definitions.lbignum
+
+[@@ Comment "Write `a + b mod 2^4096` in `res`.
+
+  This functions returns the carry.
+
+  The arguments a, b and res are meant to be 4096-bit bignums, i.e. uint64_t[64]"]
+val add: Hacl.Bignum.Addition.bn_add_eq_len_st n
+
+[@@ Comment "Write `a - b mod 2^4096` in `res`.
+
+  This functions returns the carry.
+
+  The arguments a, b and res are meant to be 4096-bit bignums, i.e. uint64_t[64]"]
+val sub: Hacl.Bignum.Addition.bn_sub_eq_len_st n
+
+[@@ Comment "Write `a * b` in `res`.
+
+  The arguments a and b are meant to be 4096-bit bignums, i.e. uint64_t[64].
+  The outparam res is meant to be a 8192-bit bignum, i.e. uint64_t[128]."]
+val mul: a:lbignum n -> b:lbignum n -> BN.bn_mul_st a b
+
+val mod_exp: BE.bn_mod_exp_st 4096ul n
